theories/Data/Fun.v
@@ -1,4 +1,5 @@
 Require Import ExtLib.Structures.Functor.
+Require Import ExtLib.Structures.Logic.
 
 Set Implicit Arguments.
 Set Strict Implicit.
@@ -8,3 +9,73 @@ Definition Fun A B := A -> B.
 Instance FunFunctor A : Functor (Fun A) :=
 { fmap _A _B g f x := g (f x)
 }.
+
+Section MonadicLogic.
+  Variables (T P : Type).
+  Context {L : Logic P}.
+
+  Global Instance Logic_Fun : Logic (T -> P) :=
+  { Entails g p := forall x, Entails (List.map (fun p => p x) g) (p x)
+  ; Tr       := fun _ => Tr
+  ; Fa       := fun _ => Fa
+  ; And  p q := fun x => And (p x) (q x)
+  ; Or   p q := fun x => Or (p x) (q x)
+  ; Impl p q := fun x => Impl (p x) (q x)
+  }.
+  
+  Context {LL : LogicLaws L}.
+
+  Global Instance LogicLaws_Over : LogicLaws Logic_Fun.
+  constructor; simpl; intros; 
+  try (solve [ apply Tr_True | apply Fa_False 
+            | eapply ImplI; eauto
+            | eapply ImplE; eauto 
+            | eapply AndI; eauto 
+            | eapply AndEL; eauto 
+            | eapply AndER; eauto 
+            | eapply OrIL; eauto
+            | eapply OrIR; eauto 
+            | eapply OrE; eauto 
+            ]).
+  eapply Assumption.
+  eapply List.in_map_iff. eexists. intuition.
+  Qed.
+End MonadicLogic.
+
+Section MonadicLogic_dep.
+  Variable T : Type.
+  Variable P : T -> Type.
+  Context {L : forall t, Logic (P t)}.
+
+  Global Instance Logic_DOver : Logic (forall t : T, P t) :=
+  { Entails g p := forall x, Entails (List.map (fun p => p x) g) (p x)
+  ; Tr       := fun _ => Tr
+  ; Fa       := fun _ => Fa
+  ; And  p q := fun x => And (p x) (q x)
+  ; Or   p q := fun x => Or (p x) (q x)
+  ; Impl p q := fun x => Impl (p x) (q x)
+  }.
+  
+  Context {LL : forall t, LogicLaws (L t)}.
+
+  Global Instance LogicLaws_DOver : LogicLaws Logic_DOver.
+  constructor; simpl; intros; 
+  try (solve [ apply Tr_True | apply Fa_False 
+            | eapply ImplI; eauto
+            | eapply ImplE; eauto 
+            | eapply AndI; eauto 
+            | eapply AndEL; eauto 
+            | eapply AndER; eauto 
+            | eapply OrIL; eauto
+            | eapply OrIR; eauto 
+            | eapply OrE; eauto 
+            ]).
+  eapply Assumption.
+  eapply List.in_map_iff. eexists. intuition.
+  Qed.
+End MonadicLogic_dep.
+
+Instance Quant_Fun (T U : Type) (Q : Quant U) : Quant (T -> U) :=
+{| All := fun V P => fun (t : T) => All (fun x : V => P x t)
+ ; Ex  := fun V P => fun (t : T) => Ex (fun x : V => P x t)
+ |}.
